intermediate/Veritas.Intermediate.TSLog.fst
@@ -88,3 +88,21 @@ let lemma_empty_implies_spec_rel (#vcfg:_) (ils:its_log vcfg{I.length ils = 0})
 let lemma_spec_rel_implies_prefix_spec_rel (#vcfg:_) (ils:its_log vcfg) (i:nat{i <= I.length ils})
  : Lemma (ensures (let ils' = I.prefix ils i in
                    spec_rel ils')) = admit()
+
+let lemma_blum_evict_def (#vcfg:_) 
+                         (ils: its_log vcfg) 
+                         (i:I.seq_index ils {is_evict_to_blum (I.index ils i)})
+  : Lemma (ensures (let be = blum_evict_elem ils i in
+                    let tid = thread_id_of ils i in
+                    let vs = thread_state_pre ils i in
+                    let st = IntV.thread_store vs in
+                    let e = I.index ils i in
+                    let s = slot_of e in
+                    inuse_slot st s /\
+                    (let k = stored_key st s in
+                     let v = stored_value st s in
+                     match e with
+                     | EvictB_S _ t -> be = MHDom (k,v) t tid
+                     | EvictBM_S _ _ t -> be = MHDom (k,v) t tid
+                    ))) = admit()
+                         
